chore: Cleanup and optimize jumping proofs (#62)

SP1Chips/JalrChip.lean
@@ -1,14 +1,13 @@
-import SP1Foundations
 import SP1Operations.Operation.AddOperation
 import SP1Operations.Reader.CPUState
 import SP1Operations.Reader.ITypeReader
-import LeanRV64IM.RiscvInstsEnd
-
 import SP1Chips.Jalr.Constraints
 
 namespace Jalr
 
 open Sail SailState BitVec LeanRV64IM.Functions
+
+variable (Main : Vector (Fin BB) 38) (s : SailState)
 
 lemma op_a_lt32_of_constraints {Main : Vector (Fin BB) 38} (h : (constraints Main).allHold)
     (h_is_real : Main[29] = 1) : Main[6].val < 2^5 := by
@@ -16,12 +15,9 @@ lemma op_a_lt32_of_constraints {Main : Vector (Fin BB) 38} (h : (constraints Mai
   have reader_cstrs := by
     simp [SP1ConstraintList.allHold, constraints, SP1Constraint.toProp] at h
     exact h.2.2.1
-  clear h
   simp [ITypeReader.constraints, h_is_real, Opcode.ofNat,
     Nat.ble, Nat.beq, SP1Constraint.toProp] at reader_cstrs
-  have trusted_instr_cstrs := reader_cstrs.1
-  clear reader_cstrs
-  itauto
+  aesop
 
 lemma op_b_lt32_of_constraints {Main : Vector (Fin BB) 38} (h : (constraints Main).allHold)
     (h_is_real : Main[29] = 1) : Main[14].val < 2^5 := by
@@ -29,45 +25,40 @@ lemma op_b_lt32_of_constraints {Main : Vector (Fin BB) 38} (h : (constraints Mai
   have reader_cstrs := by
     simp [SP1ConstraintList.allHold, constraints, SP1Constraint.toProp] at h
     exact h.2.2.1
-  clear h
   simp [ITypeReader.constraints, h_is_real, Opcode.ofNat,
     Nat.ble, Nat.beq, SP1Constraint.toProp] at reader_cstrs
-  have trusted_instr_cstrs := reader_cstrs.1
-  clear reader_cstrs
-  itauto
+  aesop
 
-variable (Main : Vector (Fin BB) 38)
-  (s : SailState) (cstrs : (constraints Main).allHold)
-  (h_is_real : Main[29] = 1)
+def sp1_op_a (cstrs : (constraints Main).allHold) (h_is_real : Main[29] = 1) : BitVec 5 :=
+  Main[6].val#'(op_a_lt32_of_constraints cstrs h_is_real)
 
-def sp1_imm : BitVec 12 := BitVec.ofNat 12 Main[21].val
+-- dt: could instead put `Word.toBitVec64 #v[Main[14], Main[15], Main[16], Main[17]]` here...
+def sp1_op_b (cstrs : (constraints Main).allHold) (h_is_real : Main[29] = 1): BitVec 5 :=
+  Main[14].val#'(op_b_lt32_of_constraints cstrs h_is_real)
 
-def sp1_op_a : BitVec 5 := Main[6].val#'(op_a_lt32_of_constraints cstrs h_is_real)
+-- dt: could instead put `Word.toBitVec64 #v[Main[21], Main[22], Main[23], Main[24]]` here...
+def sp1_op_c : BitVec 12 := BitVec.ofNat 12 Main[21].val
 
-def sp1_op_b : BitVec 5 := Main[14].val#'(op_b_lt32_of_constraints cstrs h_is_real)
-
-def sp1_jalr : SailM Unit := do
+def sp1_jalr  (cstrs : (constraints Main).allHold) (h_is_real : Main[29] = 1): SailM Unit := do
   let op_a := sp1_op_a Main cstrs h_is_real
-  write_reg op_a (Word.toBitVec64 #v[Main[34], Main[35], Main[36], Main[37]])
-  Sail.writeReg Register.nextPC (Word.toBitVec64 #v[Main[30], Main[31], Main[32], Main[33]])
+  wX_bits (.Regidx op_a) (Word.toBitVec64 #v[Main[34], Main[35], Main[36], Main[37]])
+  writeReg Register.nextPC (Word.toBitVec64 #v[Main[30], Main[31], Main[32], Main[33]])
 
 def spec_jalr (imm : BitVec 12) (rs1 rd : regidx) : SailM Unit := do
-  Sail.writeReg Register.nextPC ((← Sail.readReg Register.PC) + 4#64)
+  writeReg Register.nextPC ((← readReg Register.PC) + 4#64)
   _ ← execute_JALR imm rs1 rd
-  pure ()
-
-@[simp] lemma Opcode.ofNat_34 : Opcode.ofNat 34 = Opcode.JALR := rfl
 
 set_option debug.skipKernelTC true in
-set_option maxHeartbeats 0 in
 theorem JALR_correct
+    (cstrs : (constraints Main).allHold)
+    (h_is_real : Main[29] = 1)
     (state_cstrs : (constraints Main).initialState s)
     (h_misa : Register.misa ∈ s.regs) :
-    let imm := sp1_imm Main
     let op_b := sp1_op_b Main cstrs h_is_real
     let op_a := sp1_op_a Main cstrs h_is_real
-    (spec_jalr imm (.Regidx op_b) (.Regidx op_a)).run s = (sp1_jalr Main cstrs h_is_real).run s := by
-  extract_lets imm op_b op_a
+    let op_c := sp1_op_c Main
+    (spec_jalr op_c (.Regidx op_b) (.Regidx op_a)).run s = (sp1_jalr Main cstrs h_is_real).run s := by
+  extract_lets op_c op_b op_a
 
   -- pull out state constraints about the contents of register and pc reads
   simp [SP1ConstraintList.initialState, constraints, SP1Constraint.toStateProp, List.Forall, AddOperation.constraints, ITypeReader.constraints, CPUState.constraints, h_is_real] at state_cstrs
@@ -91,8 +82,6 @@ theorem JALR_correct
     exact Word.isU64_of_cases #v[Main[3], Main[4], Main[5], 0] h_pc_0 h_pc_1 h_pc_2 (by simp)
 
   have ⟨res_is_u64, h_res⟩ := (AddOperation.correct #v[Main[15], Main[16], Main[17], Main[18]] #v[Main[21], Main[22], Main[23], Main[24]] { value := #v[Main[30], Main[31], Main[32], Main[33]] } Main[29] h_is_real res_cstrs) b_is_u64 imm_is_u64
-  -- rw [Word.toBitVec64_LT_eq_toNat res_is_u64, Word.toBitVec64_LT_eq_toNat b_is_u64, Word.toBitVec64_LT_eq_toNat imm_is_u64] at h_res
-  -- simp [Word.toNat, h_c_1, h_c_2, h_c_3] at h_res
 
   have h_4_is_u64 : Word.isU64 #v[4,0,0,0] :=
     Word.isU64_of_cases _ (by trivial) (by trivial) (by trivial) (by trivial)
@@ -101,29 +90,18 @@ theorem JALR_correct
       Word.toBitVec64 #v[Main[21], Main[22], Main[23], Main[24]]) % 4 = 0 := by
     rw [BitVec.ofNatLT_eq_ofNat] at read_op_b'
     rw [read_op_b'] at op_b_val_plus_imm_mul4
-    simp [Word.add_toBitVec64_mod_4, Word.toBitVec64_add_mod_4] at op_b_val_plus_imm_mul4
-    simp [Word.add_toBitVec64_mod_4, Word.toBitVec64_add_mod_4]
-    exact op_b_val_plus_imm_mul4
+    simpa using op_b_val_plus_imm_mul4
 
   have hmod4 : (Word.toBitVec64 #v[Main[15], Main[16], Main[17], Main[18]] +
-                Word.toBitVec64 #v[Main[21], Main[22], Main[23], Main[24]])[1] = false := by
+      Word.toBitVec64 #v[Main[21], Main[22], Main[23], Main[24]])[1] = false := by
     refine (mul4_means_0_1_are_0 ?_).2
-    simp at hmod
-    simp [Word.add_toBitVec64_mod_4, Word.toBitVec64_add_mod_4] at hmod
-    simp [Word.toBitVec64_add_mod_4, Word.add_toBitVec64_mod_4]
-    exact hmod
-
-
-  have hmod2 : (Word.toBitVec64 #v[Main[15], Main[16], Main[17], Main[18]] +
-      Word.toBitVec64 #v[Main[21], Main[22], Main[23], Main[24]])[0] = 0 := by
-    refine (mul4_means_0_1_are_0 hmod).1
+    simpa using hmod
 
   clear res_cstrs reader_cstrs pc_cstrs
 
-  simp [spec_jalr, sp1_jalr, execute_JALR,
-    op_a, op_b, imm, sp1_op_a, sp1_op_b, sp1_imm, EStateM.run_bind]
-  -- `simp` refuses to apply this itself
-  rw [run_readReg]
+  simp [spec_jalr, sp1_jalr, execute_JALR, op_a, op_b, op_c,
+    sp1_op_a, sp1_op_b, sp1_op_c, EStateM.run_bind]
+  rw [run_readReg] -- `simp` refuses to apply this itself
   simp only [read_pc, hmod4, read_op_b', run_rX_bits, get_reg?_insert_nextPC, ext_control_check_addr,
     Sail.BitVec.access, bit_to_bool, Sail.BitVec.update, Sail.BitVec.updateSubrange',
     bits_of_virtaddr, BitVec.reduceAllOnes, BitVec.truncate_eq_setWidth, BitVec.reduceSetWidth,
@@ -133,16 +111,14 @@ theorem JALR_correct
     run_bool_bit_backwards, Bool.false_and, EStateM.run_map, run_writeReg, EStateM.Result.map_ok,
     currentlyEnabled, hartSupports, Bool.false_and, Bool.false_or, Bool.and_self,
     BitVec.ofNat_eq_ofNat, bind_pure_comp, Functor.map_map, EStateM.run_map,
-    sign_extend,
-    Sail.BitVec.signExtend, ← h_c_sign_extend]
+    sign_extend, Sail.BitVec.signExtend, ← h_c_sign_extend]
   rw [map_const_run_readReg _ _ (by simp [h_misa])]
   simp only
   rw [run_readReg]
   simp only [Std.ExtDHashMap.get?_insert_self, run_wX_bits, BitVec.ofNat_eq_ofNat, EStateM.Result.map_ok]
 
-  -- stop
   cases op_a_0_is_bool with
-  | inl op_a_0_is_0 => {
+  | inl op_a_0_is_0 =>
     have h6 : Main[6] ≠ 0 := by simp_all
     have h6' : ∀ p : ↑Main[6] < 2 ^ 5, (BitVec.ofNatLT Main[6].val p : BitVec 5) ≠ 0#5 := by
       refine fun p h => h6 ?_
@@ -151,25 +127,21 @@ theorem JALR_correct
       simpa using h
     simp only [h6', ↓reduceIte, LawfulMonadStateOf.insert_insert_insert_cancel,
       EStateM.Result.ok.injEq, _root_.and_self, and_true, true_and]
-    rw [BitVec.helper hmod, h_res]
+    rw [BitVec.twoPow64_and_eq_self hmod, h_res]
     simp
     refine congr_fun ?_ _
     have htemp : Main[29] - Main[13] = 1 := by simp [op_a_0_is_0, h_is_real]
     have := AddOperation.correct _ _ _ _ htemp inc_pc_cstrs
-    specialize this pc_is_u64 h_4_is_u64
-    rw [this.2]
+    rw [(this pc_is_u64 h_4_is_u64).2]
     simp [BitVec.ofNat, Word.toBitVec64, Word.toNat]
-    rfl
-  }
-  | inr op_a_0_is_1 => {
+  | inr op_a_0_is_1 =>
     have h6 : Main[6] = 0 := by simp_all
     have hl : Word.toBitVec64 #v[Main[34], Main[35], Main[36], Main[37]] = 0#64 := by
       simp [op_a_0_is_1, sub_eq_zero] at chip_cstrs
       obtain ⟨_, _, ⟨ha, hb, hc, hd⟩⟩ := chip_cstrs
       simp [ha, hb, hc, hd, Word.toBitVec64, ← BitVec.toFin_inj, Word.toNat]
     simp [h6, hl]
-    rw [h_res, BitVec.helper hmod]
-  }
+    rw [h_res, BitVec.twoPow64_and_eq_self hmod]
 
 -- #print axioms Jalr.JALR_correct
 
